compcertox/TensorComp.v
@@ -76,3 +76,61 @@ Section COMP.
     |}.
 
 End COMP.
+
+(* This module defines tensor produce specific to layers. This is the same as the general one defined above
+   where the outgoing language interface replaced by li_null. Later, we expect
+   to find a trick to let Coq identify li_null and li_null@K  *)
+Module Tensor.
+  (* TODO: notation precedence *)
+  Section COMP.
+    Context {I} (K: I -> Type)
+            {li} (L: forall i, semantics li_null (li@(K i))).
+
+    Notation Ki := (forall i, K i).
+
+    Section WITH_SE.
+      Context (se: Genv.symtbl).
+
+      Variant tensor_state :=
+        tensor_st (i: I) (s:  Smallstep_.state (L i)) (k: Ki).
+
+      Inductive tensor_step: tensor_state -> trace -> tensor_state -> Prop :=
+      | step_intro i s t s' k:
+          Step (L i se) s t s' ->
+          tensor_step (tensor_st i s k) t (tensor_st i s' k).
+
+      Inductive tensor_initial_state: query (li@Ki) -> tensor_state -> Prop :=
+      | initial_state_intro i s k q:
+          initial_state (L i se) (q, k i) s ->
+          tensor_initial_state (q, k) (tensor_st i s k).
+
+      Inductive tensor_at_external: tensor_state -> query li_null -> Prop := .
+
+      Inductive tensor_after_external:
+        tensor_state -> reply li_null -> tensor_state -> Prop := .
+
+      Inductive tensor_final_state: tensor_state -> reply (li@Ki) -> Prop :=
+      | final_state_intro i s k k' r kr:
+          (forall j, i <> j -> k j = k' j) -> k' i = kr ->
+          final_state (L i se) s (r, kr) ->
+          tensor_final_state (tensor_st i s k) (r, k').
+
+    End WITH_SE.
+
+    Program Definition tensor_semantics' sk: semantics li_null (li@Ki) :=
+      {|
+      activate se :=
+        {|
+          step ge := tensor_step se;
+          initial_state := tensor_initial_state se;
+          at_external := tensor_at_external;
+          after_external := tensor_after_external;
+          final_state := tensor_final_state se;
+          globalenv := tt;
+        |};
+      skel := sk;
+      footprint id := exists i, footprint (L i) id;
+      |}.
+
+  End COMP.
+End Tensor.
